All pure part are ported to Coq 8.5

graph/FiniteGraph.v
@@ -21,7 +21,7 @@ Class LocalFiniteGraph (pg: PreGraph V E) :=
   local_enumerable: forall x, Enumerable E (out_edges pg x)
 }.
 
-Definition edge_func (pg: PreGraph V E) {lfg: LocalFiniteGraph pg} x := projT1 (local_enumerable x).
+Definition edge_func (pg: PreGraph V E) {lfg: LocalFiniteGraph pg} x := proj1_sig (local_enumerable x).
 
 Lemma edge_func_spec: forall {pg : PreGraph V E} {lfg: LocalFiniteGraph pg} e x,
   In e (edge_func pg x) <-> evalid pg e /\ src pg e = x.
@@ -291,13 +291,13 @@ Proof.
       right; auto.
     - destruct IHS as [l2 ?H].
       destruct (construct_reachable_list g a (V_DEC a (or_introl eq_refl))) as [l1 ?H].
-      exists (remove_dup equiv_dec (l1 ++ l2)).
-      split; [apply remove_dup_nodup |].
+      exists (nodup equiv_dec (l1 ++ l2)).
+      split; [apply NoDup_nodup |].
       destruct H as [_ ?].
       destruct H0 as [_ ?].
       unfold reachable_set_list, reachable_list in *.
       intros.
-      rewrite <- remove_dup_in_inv.
+      rewrite nodup_In.
       rewrite in_app_iff, reachable_through_set_eq.
       specialize (H x).
       specialize (H0 x).
